coq/cpdt/coind_sem.v
@@ -1,0 +1,68 @@
+Require Import Arith.
+
+Definition Var := nat.
+
+Definition Env := Var -> nat.
+
+Definition empty : Env := fun v => 0.
+
+Definition update (env:Env) (v:Var) (n:nat) : Env :=
+    fun (x:Var) => if beq_nat x v then n else env x.
+
+Inductive Exp : Set :=
+| EConst : nat -> Exp
+| EVar   : Var -> Exp
+| EPlus  : Exp -> Exp -> Exp
+.
+
+(* interpreter fixes the semantics *)
+Fixpoint evalExp (env:Env) (e:Exp) : nat :=
+    match e with
+    | EConst n      => n
+    | EVar v        => env v
+    | EPlus e1 e2   => evalExp env e1 + evalExp env e2
+    end.
+
+Example test_evalExp1 : evalExp empty (EConst 5) = 5.
+Proof. reflexivity. Qed.
+
+Example test_evalExp2 : evalExp (update empty 3 12) (EVar 3) = 12.
+Proof. reflexivity. Qed.
+
+Example test_evalExp3 : evalExp (update empty 3 12)(EPlus(EConst 5)(EVar 3)) = 17.
+Proof. reflexivity. Qed.
+
+
+Inductive Cmd : Set :=
+| CAssign : Var -> Exp -> Cmd
+| CSeq    : Cmd -> Cmd -> Cmd
+| CWhile  : Exp -> Cmd -> Cmd
+.
+
+
+CoInductive evalCmd : Env -> Cmd -> Env -> Prop :=
+| EvalAssign : forall (env:Env) (v:Var) (e:Exp), 
+    evalCmd env (CAssign v e) (update env v (evalExp env e))
+| EvalSeq : forall (e1 e2 e3:Env) (c1 c2:Cmd),
+    evalCmd e1 c1 e2 -> evalCmd e2 c2 e3 -> evalCmd e1 (CSeq c1 c2) e3
+| EvalWhileFalse : forall (env:Env) (e:Exp) (c:Cmd),
+    evalExp env e = 0 -> evalCmd env (CWhile e c) env
+| EvalWhileTrue : forall (e1 e2 e3:Env) (e:Exp) (c:Cmd),
+    evalExp e1 e <> 0 -> evalCmd e1 c e2 -> evalCmd e2 (CWhile e c) e3 -> 
+        evalCmd e1 (CWhile e c) e3
+.
+
+(* Need to build a coinduction principle for evalCmd *)
+Theorem evalCmd_coind : forall (R:Env -> Cmd -> Env -> Prop),
+    (forall (e1 e2:Env) (e:Exp) (v:Var), 
+        R e1 (CAssign v e) e2 -> e2 = update e1 v (evalExp e1 e))    ->
+    (forall (e1 e2 e3:Env) (c1 c2:Cmd),
+        R e1 (CSeq c1 c2) e3 -> exists e2, R e1 c1 e2 /\ R e2 c2 e3) -> 
+    (forall (e1 e2 e3:Env) (e:Exp) (c:Cmd),
+        R e1 (CWhile e c) e3 -> (evalExp e1 e = 0 /\ e3 = e1) \/ 
+        (exists (e2:Env), 
+            evalExp e1 e <> 0 /\ R e1 c e2 /\ R e2 (CWhile e c) e3)) ->
+    (forall (e1 e2:Env) (c:Cmd), R e1 c e2 -> evalCmd e1 c e2).
+Proof.
+
+Show.
