coq/eta.v
@@ -1,0 +1,24 @@
+Lemma eta_eq : forall (a b:Type) (f:a -> b), f = (fun (x:a) => f x).
+Proof.
+    intros a b f. reflexivity.
+Qed.
+
+Inductive Void : Type :=.
+
+Definition absurd (a:Type) : Void -> a :=
+    fun (x:Void) => match x with end.
+
+Lemma absurd_unique1 : forall (a:Type) (f:Void -> a) (y:a) (x:Void), y = f x.
+Proof.
+    intros a f y x. inversion x.
+Qed.
+
+
+Lemma absurd_unique2 : forall (a:Type) (f:Void -> a),
+(fun (x:Void) => f x) = (fun (x:Void) => match x with end).
+Proof.
+    intros a f. 
+
+Show.
+
+
